AstToCfgCorrectness.dfy
@@ -1,0 +1,124 @@
+include "AstToCfg_simple.dfy"
+
+
+module AstToCfgCorrectness
+{
+  import opened AstToCfg
+  import opened BoogieLang
+  import opened BoogieSemantics
+  import opened BoogieCfg
+  import opened Wrappers
+
+  lemma AstToCfgAcyclicTemp(
+    c: Cmd, 
+    nextVersion: BlockId)
+    requires NoBreaksScopesLoops(c)
+    ensures  
+      var (cfg, nextVersion', exitOpt) := AstToCfgAux(c, nextVersion); 
+      IsAcyclic(cfg.successors, cfg.entry, CoveringSet2(nextVersion, nextVersion', {exitOpt.value}))
+
+  lemma WpCfgCoverIndep<A(!new)>(a: absval_interp<A>, cfg: Cfg, n: BlockId, post: Predicate<A>, cover1: set<BlockId>, cover2: set<BlockId>)
+    requires cfg.successors.Keys <= cfg.blocks.Keys
+    requires IsAcyclic(cfg.successors, n, cover1)
+    requires IsAcyclic(cfg.successors, n, cover2)
+    ensures WpCfg(a, cfg, n, post, cover1) == WpCfg(a, cfg, n, post, cover2)
+   
+  lemma AstToCfgSemanticsPreservation<A(!new)>(
+    a: absval_interp<A>,
+    c: Cmd, 
+    nextVersion: BlockId,
+    post: WpPostShallow<A>,
+    s: state<A>)
+    requires NoBreaksScopesLoops(c)
+    ensures 
+      var (cfg, nextVersion', exitOpt):= AstToCfgAux(c, nextVersion); 
+      var exit := exitOpt.value;
+      var cover' := CoveringSet2(nextVersion, nextVersion', {exitOpt.value});
+
+      assume LabelsWellDefAux(c, post.scopes.Keys); 
+      assume IsAcyclic(cfg.successors, cfg.entry, CoveringSet2(nextVersion, nextVersion', {exitOpt.value}));
+      WpShallow(a, c, post)(s) == WpCfg(a, cfg, cfg.entry, post.normal, cover')(s)
+    {
+      match c {
+        case SimpleCmd(sc) => 
+        case Seq(c1, c2) =>
+          var (cfg1, nextVersion1, exitOpt1) := AstToCfgAux(c1, nextVersion);
+          var exit1 := exitOpt1.value;
+          
+          var (cfg2, nextVersion2, exitOpt2) := AstToCfgAux(c2, nextVersion1);
+          var exit2 := exitOpt2.value; 
+
+          var cover1 := CoveringSet2(nextVersion, nextVersion1, {exitOpt1.value});
+          var cover2 := CoveringSet2(nextVersion1, nextVersion2, {exitOpt2.value});
+          var cover3 := CoveringSet2(nextVersion, nextVersion2, {exitOpt2.value});
+          assert cover1 + cover2 <= cover3;
+
+          var successors := (cfg1.successors + cfg2.successors)[exitOpt1.value := [cfg2.entry]];
+
+          assert successors == (cfg1.successors[exitOpt1.value := [cfg2.entry]] + cfg2.successors);
+
+          var cfg1' := Cfg(cfg1.entry, cfg1.blocks, cfg1.successors[exitOpt1.value := [cfg2.entry]]);
+
+          var cfg' := Cfg(cfg1.entry, cfg1.blocks + cfg2.blocks, successors);
+
+          AstToCfgAcyclicTemp(c1, nextVersion);
+          AstToCfgAcyclicTemp(c2, nextVersion1);
+
+          assume LabelsWellDefAux(c, post.scopes.Keys); 
+
+          AstToCfgAcyclicTemp(c1, nextVersion);
+          AstToCfgAcyclicTemp(c2, nextVersion1);
+          AstToCfgAcyclicTemp(c, nextVersion);
+          
+          calc {
+            WpShallow(a, c, post)(s);
+            WpShallow(a, Seq(c1,c2), post)(s); //normal definition
+            WpShallow(a, c1, WpPostShallow(WpShallow(a, c2, post), post.currentScope, post.scopes))(s); //IH
+            WpCfg(a, cfg1, cfg1.entry, WpShallow(a, c2, post), cover1)(s); //IH + pointwise
+            {
+              forall s' | true
+              ensures WpShallow(a, c2, post)(s') == WpCfg(a, cfg2, cfg2.entry, post.normal, cover2)(s')
+              { 
+                AstToCfgSemanticsPreservation(a, c2, nextVersion1, post, s');
+              }
+              WpCfgPointwise(a, cfg1, cfg1.entry, WpShallow(a, c2, post), WpCfg(a, cfg2, cfg2.entry, post.normal, cover2), cover1, s);
+            }
+            WpCfg(a, cfg1, cfg1.entry, WpCfg(a, cfg2, cfg2.entry, post.normal, cover2), cover1)(s); 
+              { 
+                assert cfg1.blocks.Keys == cfg1.successors.Keys + {exitOpt1.value};
+                assert cfg2.blocks.Keys == cfg2.successors.Keys + {exitOpt2.value};
+                assert cfg1.successors.Keys <= CoveringSet2(nextVersion, nextVersion1, {exit1});
+                assert cfg2.successors.Keys <= CoveringSet2(nextVersion1, nextVersion2, {exit1});
+                assert CoveringSet2(nextVersion, nextVersion1, {}) !! CoveringSet2(nextVersion1, nextVersion2, {});
+                AstToCfgAcyclic(c1, nextVersion);
+
+                assert IsAcyclic(cfg1.successors, cfg1.entry, cover1);
+
+                assert IsAcyclic(cfg1.successors[exit1 := [cfg2.entry]], cfg1.entry, cover1 + {exit1}) by {
+                  IsAcyclicUpdate2(cfg1.successors, cfg1.entry, exit1, [cfg2.entry], cover1);
+                }
+
+                AstToCfgAcyclic(c2, nextVersion1);
+
+                assert IsAcyclic(cfg2.successors, cfg2.entry, cover2);
+
+                  IsAcyclicMerge(
+                    cfg1.successors[exit1 := [cfg2.entry]], cfg2.successors, cfg1.entry, cfg2.entry, 
+                    cover1+{exit1},
+                    cover2
+                  );
+
+                assert (cover1+{exit1})+cover2 == cover1+cover2+{exit1};
+                WpCfgMerge(a, cfg1, cfg2, cfg1.entry, exit1, post.normal, cover1, cover2, s);
+
+                assert cover3 == cover1+cover2+{exit1};
+              }
+            WpCfg(a, cfg', cfg1.entry, post.normal, cover3)(s);
+          }
+        case _ => assume false;
+      }
+
+    }
+
+}
+
